dot_storeless_subst_aux: add option-less par. substitution w/ lemmas
I reproved all lemmas in this file pretty quickly (a few hours of work) and most
proofs are easier. Not sure this interface is ideal tho.

ecoop17/dot_storeless_subst_aux.v
@@ -129,6 +129,52 @@ Hint Resolve steps_irred_det.
 
 Require Import dot_monads.
 
+Fixpoint vr_subst_par (sigma: id -> vr) (v: vr) { struct v }: vr :=
+  match v with
+    | VarF x => sigma x
+    | VarB x => VarB x
+    | VObj dms =>
+      VObj (dms_subst_par sigma dms)
+  end
+with subst_par (sigma: id -> vr) (T: ty) { struct T }: ty :=
+  match T with
+    | TTop        => TTop
+    | TBot        => TBot
+    | TSel v1 l     =>
+      TSel (vr_subst_par sigma v1) l
+    | TFun l T1 T2  =>
+      TFun l (subst_par sigma T1) (subst_par sigma T2)
+    | TMem l T1 T2  =>
+      TMem l (subst_par sigma T1) (subst_par sigma T2)
+    | TBind T1    =>
+      TBind (subst_par sigma T1)
+    | TAnd T1 T2  =>
+      TAnd (subst_par sigma T1) (subst_par sigma T2)
+    | TOr T1 T2   =>
+      TOr (subst_par sigma T1) (subst_par sigma T2)
+    | TLater T1    =>
+      TLater (subst_par sigma T1)
+  end
+with tm_subst_par (sigma: id -> vr) (t: tm) { struct t }: tm :=
+   match t with
+     | tvar v =>
+       tvar (vr_subst_par sigma v)
+     | tapp t1 l t2 =>
+       tapp (tm_subst_par sigma t1) l (tm_subst_par sigma t2)
+   end
+with dm_subst_par (sigma: id -> vr) (d: dm) { struct d }: dm :=
+   match d with
+     | dfun T1 T2 t2 =>
+       dfun (subst_par sigma T1) (subst_par sigma T2) (tm_subst_par sigma t2)
+     | dty T1 =>
+       dty (subst_par sigma T1)
+   end
+with dms_subst_par (sigma: id -> vr) (ds: dms) { struct ds }: dms :=
+   match ds with
+     | dnil => dnil
+     | dcons d ds =>
+       dcons (dm_subst_par sigma d) (dms_subst_par sigma ds)
+   end.
 
 Lemma Forall_map: forall {X Y} (xs: list X) (f: X -> Y) (P : X -> Prop) (Q : Y -> Prop),
     Forall P xs ->
@@ -142,6 +188,82 @@ Lemma dms_to_env_closed: forall i k env,
     Forall (vr_closed i k) (map VObj env).
 Proof. eauto using Forall_map. Qed.
 Hint Resolve dms_to_env_closed.
+
+Fixpoint env_to_sigma (env: list vr) (n: id): vr :=
+  match env with
+    | [] => VarF n
+    | x :: xs  => if beq_nat n (length xs) then x else env_to_sigma xs n
+  end.
+
+Lemma env_to_sigma_index (env: list vr): forall n, n < length env -> index n env = Some (env_to_sigma env n).
+Proof.
+  induction env; simpl; intros;
+    [ omega | better_case_match; beq_nat; eauto ].
+Qed.
+
+Lemma env_to_sigma_Forall:
+  forall (env : list vr) i P, Forall P env -> i < length env ->
+                            P (env_to_sigma env i).
+Proof.
+  intros * HFor Hlen; induction env; cbn in *.
+  - omega.
+  - inverse HFor; case_match; beq_nat; eauto.
+Qed.
+
+(* Use "solve" because in subst_all_res_closed_rec this tactic leads the proof
+   search down the wrong path whenever it doesn't solve the goal immediately;
+   using "solve" is sort of what eauto's proof search and backtracking would do
+   anyway: if applying this lemma and searching further doesn't help, backtrack. *)
+Ltac apply_env_Forall :=
+  match goal with
+  | H: Forall ?P ?env |- ?P _ => try solve [eapply (env_to_sigma_Forall _ _ _ H); eauto]
+  end.
+
+(* Seems to actually work fine, but this is needed too seldom for now, and can be expensive. *)
+(* Hint Extern 5 => apply_Forall. *)
+Lemma subst_par_nonTot_res_closed_rec:
+  (forall v, forall i k env, Forall (vr_closed i k) env -> vr_closed (length env) k v ->
+                   vr_closed i k (vr_subst_par (env_to_sigma env) v)) /\
+  (forall T, forall i k env, Forall (vr_closed i k) env -> closed (length env) k T ->
+                   closed i k (subst_par (env_to_sigma env) T)) /\
+  (forall t, forall i k env, Forall (vr_closed i k) env -> tm_closed (length env) k t ->
+                   tm_closed i k (tm_subst_par (env_to_sigma env) t)) /\
+  (forall d, forall i k env, Forall (vr_closed i k) env -> dm_closed (length env) k d ->
+                   dm_closed i k (dm_subst_par (env_to_sigma env) d)) /\
+  (forall d, forall i k env, Forall (vr_closed i k) env -> dms_closed (length env) k d ->
+                   dms_closed i k (dms_subst_par (env_to_sigma env) d)).
+Proof.
+  apply syntax_mutind; simpl; intros; inverts_closed;
+    apply_env_Forall || eauto 7.
+Qed.
+
+Lemma vr_subst_par_nonTot_res_closed:
+  (forall v i k env, Forall (vr_closed i k) env -> forall (Hcl: vr_closed (length env) k v),
+        vr_closed i k (vr_subst_par (env_to_sigma env) v)).
+Proof. unmut_lemma subst_par_nonTot_res_closed_rec. Qed.
+Lemma subst_par_nonTot_res_closed:
+  (forall T i k env, Forall (vr_closed i k) env -> forall (Hcl: closed (length env) k T),
+        closed i k (subst_par (env_to_sigma env) T)).
+Proof. unmut_lemma subst_par_nonTot_res_closed_rec. Qed.
+Lemma tm_subst_par_nonTot_res_closed:
+  (forall t i k env, Forall (vr_closed i k) env -> forall (Hcl: tm_closed (length env) k t),
+        tm_closed i k (tm_subst_par (env_to_sigma env) t)).
+Proof. unmut_lemma subst_par_nonTot_res_closed_rec. Qed.
+Lemma dm_subst_par_nonTot_res_closed:
+  (forall d i k env, Forall (vr_closed i k) env -> forall (Hcl: dm_closed (length env) k d),
+        dm_closed i k (dm_subst_par (env_to_sigma env) d)).
+Proof. unmut_lemma subst_par_nonTot_res_closed_rec. Qed.
+Lemma dms_subst_par_nonTot_res_closed:
+  (forall d i k env, Forall (vr_closed i k) env -> forall (Hcl: dms_closed (length env) k d),
+        dms_closed i k (dms_subst_par (env_to_sigma env) d)).
+Proof. unmut_lemma subst_par_nonTot_res_closed_rec. Qed.
+Hint Resolve
+     vr_subst_par_nonTot_res_closed
+     subst_par_nonTot_res_closed
+     tm_subst_par_nonTot_res_closed
+     dm_subst_par_nonTot_res_closed
+     dms_subst_par_nonTot_res_closed.
+
 Fixpoint vr_subst_all (env: list vr) (v: vr) { struct v }: option vr :=
   match v with
     | VarF x => index x env
@@ -269,6 +391,11 @@ Hint Resolve
 Definition evalToSome env e v k j :=
   (exists t', tm_subst_all (map VObj env) e = Some t' /\ steps t' v j) /\ irred v /\ j <= k.
 
+Notation dmEnv_to_sigma env := (env_to_sigma (map VObj env)).
+
+Definition evalToSomePar env e v k j :=
+  steps (tm_subst_par (dmEnv_to_sigma env) e) v j /\ irred v /\ j <= k.
+
 Lemma evalToSomeRes_closed: forall env e v n k j l,
     evalToSome env e v n j ->
     tm_closed l 0 e ->
@@ -284,10 +411,24 @@ Proof.
 Qed.
 Hint Resolve evalToSomeRes_closed.
 
+Lemma evalToSomeParRes_closed: forall env e v n k j l,
+    evalToSomePar env e v n j ->
+    tm_closed l 0 e ->
+    length env = l ->
+    Forall (dms_closed k 1) env ->
+    tm_closed k 0 v.
+Proof.
+  unfold evalToSomePar; intros; subst; ev;
+    eapply steps_closed; eauto;
+      eapply tm_subst_par_nonTot_res_closed; try rewrite map_length; eauto.
+Qed.
+Hint Resolve evalToSomeParRes_closed.
+
 (*******************)
 (* Prove irreducible closed terms evaluate to themselves (vl_evalToSome_self).
    We must first prove that substitution leaves them unchnaged. *)
 
+Definition vr_env_id_par xs := forall n, env_to_sigma xs n = VarF n.
 (* Define what's an identity substitution, through the required property (rather than through an inductive type). *)
 Definition vr_env_id xs := forall n, n < length xs -> index n xs = Some (VarF n).
 
@@ -296,10 +437,17 @@ Definition vr_env_id xs := forall n, n < length xs -> index n xs = Some (VarF n)
 Lemma nil_vr_env_id: vr_env_id [].
 Proof. unfold vr_env_id; simpl; easy. Qed.
 
+Lemma nil_vr_env_id_par: vr_env_id_par [].
+Proof. red. reflexivity. Qed.
+
 Lemma cons_vr_env_id: forall env, vr_env_id env -> vr_env_id (VarF (length env) :: env).
 Proof. unfold vr_env_id; simpl; intros; case_match; beq_nat; subst; auto. Qed.
 
+Lemma cons_vr_env_id_par: forall env, vr_env_id_par env -> vr_env_id_par (VarF (length env) :: env).
+Proof. unfold vr_env_id_par; simpl; intros; better_case_match; beq_nat; auto. Qed.
+
 Hint Resolve nil_vr_env_id cons_vr_env_id.
+Hint Resolve nil_vr_env_id_par cons_vr_env_id_par.
 
 (* Prove that an identity substitution is also an identity when lifted to our
    language syntax. *)
@@ -367,14 +515,82 @@ Lemma dms_subst_closed_id:
 Proof. unmut_lemma subst_closed_id_rec. Qed.
 Hint Resolve vr_subst_closed_id subst_closed_id tm_subst_closed_id dm_subst_closed_id dms_subst_closed_id.
 
+Lemma subst_par_closed_id_rec:
+  (forall v i l env, vr_env_id_par env ->
+              l = length env ->
+              vr_closed l i v ->
+              vr_subst_par (env_to_sigma env) v = v) /\
+  (forall T i l env, vr_env_id_par env ->
+              l = length env ->
+              closed l i T ->
+              subst_par (env_to_sigma env) T = T) /\
+  (forall t i l env, vr_env_id_par env ->
+              l = length env ->
+              tm_closed l i t ->
+              tm_subst_par (env_to_sigma env) t = t) /\
+  (forall d i l env, vr_env_id_par env ->
+              l = length env ->
+              dm_closed l i d ->
+              dm_subst_par (env_to_sigma env) d = d) /\
+  (forall d i l env, vr_env_id_par env ->
+              l = length env ->
+              dms_closed l i d ->
+              dms_subst_par (env_to_sigma env) d = d).
+Proof.
+  apply syntax_mutind;
+    simpl; intros; subst; inverts_closed; try f_equal; eauto.
+Qed.
+
+Lemma vr_subst_par_closed_id:
+  forall v i l env, vr_env_id_par env ->
+              l = length env ->
+              vr_closed l i v ->
+              vr_subst_par (env_to_sigma env) v = v.
+Proof. unmut_lemma subst_par_closed_id_rec. Qed.
+Lemma subst_par_closed_id:
+  forall T i l env, vr_env_id_par env ->
+               l = length env ->
+               closed l i T ->
+               subst_par (env_to_sigma env) T = T.
+Proof. unmut_lemma subst_par_closed_id_rec. Qed.
+Lemma tm_subst_par_closed_id:
+  forall t i l env,
+    vr_env_id_par env ->
+    l = length env ->
+    tm_closed l i t ->
+    tm_subst_par (env_to_sigma env) t = t.
+Proof. unmut_lemma subst_par_closed_id_rec. Qed.
+Lemma dm_subst_par_closed_id:
+  forall d i l env, vr_env_id_par env ->
+              l = length env ->
+              dm_closed l i d ->
+              dm_subst_par (env_to_sigma env) d = d.
+Proof. unmut_lemma subst_par_closed_id_rec. Qed.
+Lemma dms_subst_par_closed_id:
+  forall d i l env, vr_env_id_par env ->
+              l = length env ->
+              dms_closed l i d ->
+              dms_subst_par (env_to_sigma env) d = d.
+Proof. unmut_lemma subst_par_closed_id_rec. Qed.
+Hint Resolve vr_subst_par_closed_id subst_par_closed_id tm_subst_par_closed_id dm_subst_par_closed_id dms_subst_par_closed_id.
+
 Lemma tm_subst_closed_id_nil: forall t i, tm_closed 0 i t -> tm_subst_all [] t = Some t.
 Proof. eauto. Qed.
 Hint Resolve tm_subst_closed_id_nil.
+
+Lemma tm_subst_par_closed_id_nil: forall t i, tm_closed 0 i t -> tm_subst_par (env_to_sigma []) t = t.
+Proof. eauto. Qed.
+Hint Resolve tm_subst_par_closed_id_nil.
 
 Hint Constructors steps.
 
 Lemma vl_evalToSome_self: forall v n i, irred v -> tm_closed 0 i v -> evalToSome [] v v n 0.
 Proof. unfold evalToSome; intuition eauto. Qed.
+
+Lemma vl_evalToSomePar_self: forall v n i, irred v -> tm_closed 0 i v -> evalToSomePar [] v v n 0.
+Proof.
+  unfold evalToSomePar; intuition (try erewrite tm_subst_par_closed_id_nil; eauto).
+Qed.
 
 Lemma evalToSome_det: forall env e k j1 j2 {v1} {v2},
     evalToSome env e v1 k j1 ->
@@ -382,6 +598,13 @@ Lemma evalToSome_det: forall env e k j1 j2 {v1} {v2},
     v1 = v2 /\ j1 = j2.
 Proof. unfold evalToSome; intros; ev; optFuncs_det; eapply steps_irred_det; eauto. Qed.
 Hint Resolve evalToSome_det.
+
+Lemma evalToSomePar_det: forall env e k j1 j2 {v1} {v2},
+    evalToSomePar env e v1 k j1 ->
+    evalToSomePar env e v2 k j2 ->
+    v1 = v2 /\ j1 = j2.
+Proof. unfold evalToSomePar; intros; ev; eauto. Qed.
+Hint Resolve evalToSomePar_det.
 
 Lemma subst_all_upgrade_rec:
   (forall v v' env vx i l, vr_subst_all env v = Some v' ->
@@ -452,6 +675,65 @@ Proof. unmut_lemma subst_all_upgrade_rec. Qed.
 
 Hint Resolve vr_subst_all_upgrade subst_all_upgrade tm_subst_all_upgrade dm_subst_all_upgrade dms_subst_all_upgrade.
 
+Lemma subst_par_upgrade_rec:
+  (forall v v' env vx i l, vr_subst_par (env_to_sigma env) v = v' ->
+                    vr_closed l i v ->
+                    length env = l ->
+                    vr_subst_par (env_to_sigma (vx :: env)) v = v') /\
+  (forall T T' env vx i l, subst_par (env_to_sigma env) T = T' ->
+                    closed l i T ->
+                    length env = l ->
+                    subst_par (env_to_sigma (vx :: env)) T = T') /\
+  (forall t t' env vx i l, tm_subst_par (env_to_sigma env) t = t' ->
+                    tm_closed l i t ->
+                    length env = l ->
+                    tm_subst_par (env_to_sigma (vx :: env)) t = t') /\
+  (forall d d' env vx i l, dm_subst_par (env_to_sigma env) d = d' ->
+                    dm_closed l i d ->
+                    length env = l ->
+                    dm_subst_par (env_to_sigma (vx :: env)) d = d') /\
+  (forall d d' env vx i l, dms_subst_par (env_to_sigma env) d = d' ->
+                    dms_closed l i d ->
+                    length env = l ->
+                    dms_subst_par (env_to_sigma (vx :: env)) d = d').
+Proof.
+  apply syntax_mutind; simpl; intros; inverts_closed; injectHyps; subst.
+  all: try solve [f_equal; eauto | case_match; beq_nat; subst; omega || trivial ].
+Qed.
+
+Lemma vr_subst_par_upgrade:
+  forall v v' env vx i l, vr_subst_par (env_to_sigma env) v = v' ->
+                   vr_closed l i v ->
+                   length env = l ->
+                   vr_subst_par (env_to_sigma (vx :: env)) v = v'.
+Proof. unmut_lemma subst_par_upgrade_rec. Qed.
+Lemma subst_par_upgrade:
+  forall T T' env vx i l, subst_par (env_to_sigma env) T = T' ->
+                   closed l i T ->
+                   length env = l ->
+                   subst_par (env_to_sigma (vx :: env)) T = T'.
+Proof. unmut_lemma subst_par_upgrade_rec. Qed.
+Lemma tm_subst_par_upgrade:
+  forall t t' env vx i l, tm_subst_par (env_to_sigma env) t = t' ->
+                   tm_closed l i t ->
+                   length env = l ->
+                   tm_subst_par (env_to_sigma (vx :: env)) t = t'.
+Proof. unmut_lemma subst_par_upgrade_rec. Qed.
+Lemma dm_subst_par_upgrade:
+  forall d d' env vx i l, dm_subst_par (env_to_sigma env) d = d' ->
+                   dm_closed l i d ->
+                   length env = l ->
+                   dm_subst_par (env_to_sigma (vx :: env)) d = d'.
+Proof. unmut_lemma subst_par_upgrade_rec. Qed.
+Lemma dms_subst_par_upgrade:
+  forall d d' env vx i l, dms_subst_par (env_to_sigma env) d = d' ->
+                   dms_closed l i d ->
+                   length env = l ->
+                   dms_subst_par (env_to_sigma (vx :: env)) d = d'.
+Proof. unmut_lemma subst_par_upgrade_rec. Qed.
+
+Hint Resolve vr_subst_par_upgrade subst_par_upgrade tm_subst_par_upgrade dm_subst_par_upgrade dms_subst_par_upgrade.
+
 Lemma subst_env: forall v v' env, tm_subst_all [] v = Some v' ->
                              tm_closed 0 0 v ->
                              tm_subst_all env v = Some v'.
@@ -459,3 +741,11 @@ Proof.
   specialize tm_subst_all_upgrade with (i := 0); induction env; intuition eauto.
 Qed.
 Hint Resolve subst_env.
+
+Lemma subst_par_env: forall v v' env, tm_subst_par (env_to_sigma []) v = v' ->
+                             tm_closed 0 0 v ->
+                             tm_subst_par (env_to_sigma env) v = v'.
+Proof.
+  specialize tm_subst_par_upgrade with (i := 0); induction env; intuition eauto.
+Qed.
+Hint Resolve subst_par_env.
